refactor(core,rust_primitives): reoganize & remove `assume`s

examples/core/Core.Ops.Range.RangeTo.fst
@@ -1,6 +1,0 @@
-module Core.Ops.Range.RangeTo
-open Rust_primitives
-
-
-type range = {f_end: usize}
-
