examples/rust_primitives/Rust_primitives.Arrays.fst
@@ -13,6 +13,9 @@ let to_list (#t:Type) s = Seq.seq_to_list s
 let to_of_list_lemma t l = Seq.lemma_list_seq_bij l
 let of_to_list_lemma t l = Seq.lemma_seq_list_bij l
 
+let length (arr: slice 'a): usize = sz (Seq.length arr)
+let contains (#t: eqtype) (arr: slice t) (x: t): bool = Seq.mem x arr
+
 let map_array #n (arr: t_Array 'a n) (f: 'a -> 'b): t_Array 'b n 
   = FStar.Seq.map_seq_len f arr;
     FStar.Seq.map_seq f arr 
