examples/core/Alloc.Vec.fst
@@ -1,7 +1,7 @@
 module Alloc.Vec
 open Rust_primitives
 
-unfold type t_Vec t _ = s:slice t{Seq.length s <= max_usize}
+unfold type t_Vec t (_: unit) = s:slice t{Seq.length s <= max_usize}
 
 let impl__new #t: t_Vec t () = FStar.Seq.empty
 
@@ -17,10 +17,10 @@ let impl_1__push
   (v: t_Vec 't ())// Removed: {Seq.length v + 1 <= max_usize})
   (x: 't)
    : t_Vec 't () = 
-     if Seq.length v <= max_usize then v else 
+     if Seq.length v <= max_usize then v else
      FStar.Seq.append v (FStar.Seq.create 1 x)
 
-let impl_1__len (v: t_Vec 't unit) =
+let impl_1__len (v: t_Vec 't ()) =
   let n = Seq.length v in
   assert (n <= maxint usize_inttype);
   mk_int #usize_inttype (Seq.length v)
