examples/core/Core.Iter.Adapters.Enumerate.fst
@@ -2,3 +2,4 @@ module Core.Iter.Adapters.Enumerate
 open Rust_primitives
 
 type t_Enumerate t = { iter: t; count: usize }
+
