examples/core/Core.Ops.Range.fsti
@@ -1,0 +1,101 @@
+module Core.Ops.Range
+open Rust_primitives
+
+type t_RangeTo   (t: Type) = {f_end: t}
+type t_RangeFrom (t: Type) = {f_start: t}
+type t_Range     (t: Type) = {f_start: t; f_end: t}
+
+open Core.Iter.Traits.Iterator
+
+let rec fold_range' #t
+  (min: Rust_primitives.int_t t) (max: Rust_primitives.int_t t {v min <= v max})
+  (init: 'a) (f: ('a -> i:Rust_primitives.int_t t{v i < v max /\ v i >= v min} -> 'a))
+  : Tot 'a (decreases (v max - v min))
+  = if min = max
+    then init
+    else fold_range' (add min (Rust_primitives.mk_int 1)) max (f init min) f
+
+val iterator_range_enumerate t: t_enumerate (t_Range (Rust_primitives.int_t t))
+
+instance iterator_range t: iterator (t_Range (Rust_primitives.int_t t)) = 
+  { item = Rust_primitives.int_t t;
+    next = (fun {f_start; f_end} -> 
+       if f_start >=. f_end then ({f_start; f_end}, None)
+       else ({f_start = f_start +. Rust_primitives.mk_int 0; f_end}, Some f_start)
+    );
+    contains = (fun x i -> v i < v x.f_end /\ v i >= v x.f_start);
+    fold = (fun #b r init f ->  if r.f_start >=. r.f_end then init
+                             else fold_range' r.f_start r.f_end init (fun x i -> f x i));
+    enumerate = iterator_range_enumerate t;
+  }
+
+open Core.Ops.Index
+
+instance impl_range_index_slice t len n : t_Index (array t len) (t_Range (int_t n)) = {
+  f_Output = slice t;
+  in_range = (fun (arr: array t len) {f_start; f_end} -> 
+    v f_start >= 0     /\
+    v f_start <= v len /\
+    v f_end   <= v len
+  );
+  f_index = (fun arr {f_start; f_end} -> 
+      if f_start <. f_end
+      then Seq.slice arr (v f_start) (v f_end)
+      else Seq.empty
+    );
+}
+
+instance impl_index_range_array t n : t_Index (slice t) (t_Range (int_t n)) = {
+  f_Output = slice t;
+  in_range = (fun (s: slice t) {f_start; f_end} -> 
+    let len = Rust_primitives.length s in
+    v f_start >= 0     /\
+    v f_start <= v len /\
+    v f_end   <= v len
+  );
+  f_index = (fun s {f_start; f_end} -> 
+      if f_start <. f_end
+      then Seq.slice s (v f_start) (v f_end)
+      else Seq.empty
+    );
+}
+
+(*
+
+module RangeTo = Core.Ops.Range.RangeTo
+
+instance rangeTo_index t len : index (array t len) RangeTo.range = {
+  output = slice t;
+  in_range = (fun (arr: array t len) { RangeTo.f_end } -> 
+    v f_end   <= Seq.length arr
+  );
+  (.[]) = (fun arr { f_end } -> 
+      Seq.slice arr 0 (v f_end)
+    );
+}
+
+module RangeFrom = Core.Ops.Range.RangeFrom
+
+instance rangeFrom_index t len : index (array t len) RangeFrom.range = {
+  output = slice t;
+  in_range = (fun (arr: array t len) { RangeFrom.f_start } -> 
+    v f_start < v len
+  );
+  (.[]) = (fun arr { f_start } -> 
+      Seq.slice arr (v f_start) (Seq.length arr)
+    );
+}
+
+instance rangeFrom_index_slice_usize t : index (slice t) usize = magic ()
+
+instance rangeFrom_index_slice t : index (slice t) RangeFrom.range = {
+  output = slice t;
+  in_range = (fun (arr: slice t) { RangeFrom.f_start } -> 
+    v f_start < Seq.length arr
+  );
+  (.[]) = (fun arr { f_start } -> 
+      Seq.slice arr (v f_start) (Seq.length arr)
+    );
+}
+
+*)
