examples/core/Core.Slice.Iter.fst
@@ -6,7 +6,3 @@ let t_Chunks a = slice (slice a)
 let t_ChunksExact a = slice (slice a)
 let t_Iter a = slice a
 
-
-
-// instance chunks_it a: iterator (t_Chunks a) = 
-
