examples/core/Core.Slice.fsti
@@ -1,0 +1,23 @@
+module Core.Slice
+open Rust_primitives
+
+let impl__len (s: slice 'a)
+  : len: usize {len == sz (Seq.length s)} = 
+  sz (Seq.length s)
+
+open Core.Slice.Iter
+
+val impl__chunks (x: slice 'a) (cs: usize): t_Chunks 'a
+
+let impl__iter (s: slice 't): slice 't = s
+
+val impl__chunks_exact (x: slice 'a) (cs: usize): t_ChunksExact 'a
+
+open Core.Ops.Index
+
+instance impl__index t: t_Index (slice t) usize
+  = { f_Output = t;
+      in_range = (fun (s: slice t) (i: usize) -> i <. length s);
+      f_index = (fun s i -> Seq.index s (v i));
+    }
+
